Solved universe inconsistency by changing Cito.Label to use FMapAVL instead of FMapWeakList.

platform/cito/Label.v
@@ -1,28 +1,69 @@
-Require Import FMapWeakList.
-Require Import String.
-Require Import Equalities.
-
 Set Implicit Arguments.
+
+Require Import String.
 
 Definition label := (string * string)%type.
 
-Module Key <: MiniDecidableType.
-  Definition t := label.
-  Definition eq_dec (a b : label) : {a = b} + {a <> b}.
-    destruct a.
-    destruct b.
-    destruct (string_dec s s1).
-    destruct (string_dec s0 s2).
-    left.
-    congruence.
-    right.
-    congruence.
-    right.
-    congruence.
-  Defined.
-End Key.
+Require Import OrderedType.
 
-Module Key' := Make_UDT Key.
-Module LabelMap := Make Key'.
+Module Label_as_MOT <: MiniOrderedType.
+
+  Definition t := label.
+
+  Definition eq := @eq t.
+
+  Require Import LabelMap.
+
+  Definition to_bl (lbl : t) : Labels.label := (fst lbl, Labels.Global (snd lbl)).
+
+  Definition lt (x y : t) := LabelKey.lt (to_bl x) (to_bl y).
+
+  Lemma eq_refl : forall x : t, eq x x.
+    unfold eq; eauto.
+  Qed.
+
+  Lemma eq_sym : forall x y : t, eq x y -> eq y x.
+    unfold eq; eauto.
+  Qed.
+
+  Lemma eq_trans : forall x y z : t, eq x y -> eq y z -> eq x z.
+    unfold eq; intuition.
+    congruence.
+  Qed.
+
+  Lemma lt_trans : forall x y z : t, lt x y -> lt y z -> lt x z.
+    unfold lt; intros.
+    eapply LabelKey.lt_trans; eauto.
+  Qed.
+
+  Lemma lt_not_eq : forall x y : t, lt x y -> ~ eq x y.
+    unfold lt; unfold eq; intuition.
+    subst.
+    eapply LabelKey.lt_not_eq in H.
+    contradict H.
+    unfold LabelKey.eq.
+    eauto.
+  Qed.
+
+  Definition compare : forall x y : t, Compare lt eq x y.
+    unfold lt; unfold eq.
+    intros.
+    destruct (LabelKey.compare (to_bl x) (to_bl y)).
+    econstructor 1; eauto.
+    econstructor 2; eauto.
+    unfold LabelKey.eq in *.
+    unfold to_bl in *.
+    destruct x; destruct y; simpl in *.
+    injection e; intros; subst.
+    eauto.
+    econstructor 3; eauto.
+  Defined.
+
+End Label_as_MOT.
+
+Module Label_as_OT := MOT_to_OT Label_as_MOT.
+
+Require Import FMapAVL.
+Module LabelMap := Make Label_as_OT.
 
 
