platform/cito/examples/ReturnZero.v
@@ -109,26 +109,56 @@ Definition return_zero_func_spec := func_spec (return_zero_gm :: nil) (empty _) 
 
 Notation extra_stack := 10.
 
-Require Import AutoSep.
 Require Import Malloc.
 
 Definition return_zero_topS := SPEC reserving (3 + extra_stack)
   PRE[_] mallocHeap 0
   POST[R] [| R = 0 |] * mallocHeap 0.
 
-Definition return_zero_top := bimport [[ ("return_zero", "return_zero", return_zero_func_spec)(* , "malloc"!"malloc" @ [mallocS]  *)]]
+Definition return_zero_top := bimport [[ ("return_zero", "return_zero", return_zero_func_spec)]]
   bmodule "return_zero_top" {{
     bfunction "return_zero_top"("R") [return_zero_topS]
       "R" <-- Call "return_zero"!"return_zero"(extra_stack)
-      (* "R" <-- Call "malloc"!"malloc"(0, 10) *)
       [PRE[_, R] [| R = 0 |]
        POST[R'] [| R' = R |] ];;
       Return "R"
     end
   }}.
 
-Require Import MakeADT.
-Module Import Made := MakeADT.Make(ExampleADT)(ExampleRepInv).
+Import CompileFuncSpecMake.
+Import InvMake.SemanticsMake.
+Import InvMake2.
+Import Inv.
+
+Require Import Arith.
+Require Import WordFacts.
+Require Import CompileStmtTactics.
+
+Lemma body_safe : forall env v, Safe env (Body return_zero) v.
+  intros.
+  unfold return_zero, Top.body.
+  econstructor; eauto.
+Qed.
+
+Lemma body_runsto : forall env v v', RunsTo env (Body return_zero) v v' -> sel (fst v') (RetVar return_zero) = 0 /\ snd v' = snd v.
+  intros.
+  inversion_clear H.
+  subst vs.
+  simpl.
+  split.
+  rewrite sel_upd_eq; eauto.
+  eauto.
+Qed.
+
+Ltac hiding tac :=
+  clear_imports;
+  ((let P := fresh "P" in
+    match goal with
+      | H : Safe ?fs _ _ |- _ => set (P := Safe fs) in *
+      | H : RunsTo ?fs _ _ _ |- _ => set (P := RunsTo fs) in *
+    end;
+    hiding tac;
+    subst P) || tac).
 
 Theorem return_zero_top_ok : moduleOk return_zero_top.
   vcgen.
@@ -137,6 +167,7 @@ Theorem return_zero_top_ok : moduleOk return_zero_top.
   post; sep_auto.
 
   post; sep_auto.
+
   etransitivity.
   Focus 2.
   eapply prelude_out with (ns' := "R" :: nil).
@@ -145,17 +176,6 @@ Theorem return_zero_top_ok : moduleOk return_zero_top.
 
   post; sep_auto.
 
-  Import CompileFuncSpecMake.
-  Import InvMake.SemanticsMake.
-  Import InvMake2.
-  Import Inv.
-
-  Require Import CompileStmtTactics.
-  Import LinkModuleImplsMake.CompileModuleMake.
-  Import CompileFuncMake.
-  Import CompileFuncImplMake.
-  Import CompileStmtTacticsMake.
-
   post.
   replace (locals _ _ _ _) with (locals_call ("rp" :: "R" :: nil) x1 12 
               (Regs x Sp) ("rp" :: "es" :: nil) 0 8) in H1 by eauto.
@@ -163,9 +183,9 @@ Theorem return_zero_top_ok : moduleOk return_zero_top.
                         | split; [ simpl; omega
                           | split; [ NoDup
                             | reflexivity ] ] ]).
-  evaluate auto_ext.
+  hiding ltac:(evaluate auto_ext).
   unfold name_marker.
-  step auto_ext.
+  hiding ltac:(step auto_ext).
   unfold spec_without_funcs_ok.
   post.
   descend.
@@ -176,15 +196,13 @@ Theorem return_zero_top_ok : moduleOk return_zero_top.
   Opaque allocated.
   simpl in *.
   rewrite H1 in *.
-  step auto_ext.
-  Require Import Arith.
-  Require Import WordFacts.
+  hiding ltac:(step auto_ext).
   rewrite wplus_0 in *.
   Open Scope nat.
-  replace (4 * 4) with (8 + 8).
+  replace (4 * 4) with (8 + 8) by eauto.
   rewrite natToW_plus in *.
   rewrite wplus_assoc in *.
-  step auto_ext.
+  hiding ltac:(step auto_ext).
 
   set (h0 := locals nil _ _ _) in *.
   unfold locals in h0.
@@ -205,16 +223,15 @@ Theorem return_zero_top_ok : moduleOk return_zero_top.
   simpl in h0.
   subst h0.
 
-  step auto_ext.
+  hiding ltac:(step auto_ext).
 
   rewrite mult_0_l in *.
   rewrite wplus_0 in *.
 
   Transparent allocated.
-
   simpl.
 
-  step auto_ext.
+  hiding ltac:(step auto_ext).
 
   set (lcl := locals ("rp" :: "R" :: nil) _ _ _).
   unfold locals, array.
@@ -225,22 +242,15 @@ Theorem return_zero_top_ok : moduleOk return_zero_top.
 
   replace es with ($10).
 
-  step auto_ext.
+  hiding ltac:(step auto_ext).
 
   subst es.
   sep_auto.
-  ring.
-  Lemma body_safe : forall env v, Safe env Top.body v.
-    intros.
-    unfold Top.body.
-    econstructor; eauto.
-  Qed.
-
   eapply body_safe.
   eauto.
 
-  step auto_ext.
-  step auto_ext.
+  hiding ltac:(step auto_ext).
+  hiding ltac:(step auto_ext).
 
   openhyp.
   destruct x6; simpl in *.
@@ -278,27 +288,7 @@ Theorem return_zero_top_ok : moduleOk return_zero_top.
   Transparent allocated.
   simpl.
 
-  Ltac hiding tac :=
-    clear_imports;
-    ((let P := fresh "P" in
-      match goal with
-        | H : Safe ?fs _ _ |- _ => set (P := Safe fs) in *
-        | H : RunsTo ?fs _ _ _ |- _ => set (P := RunsTo fs) in *
-      end;
-      hiding tac;
-      subst P) || tac).
-
   hiding ltac:(step auto_ext).
-
-  Lemma body_runsto : forall env v v', RunsTo env Top.body v v' -> sel (fst v') (RetVar return_zero) = 0 /\ snd v' = snd v.
-    intros.
-    inversion_clear H.
-    subst vs.
-    simpl.
-    split.
-    rewrite sel_upd_eq; eauto.
-    eauto.
-  Qed.
 
   eapply body_runsto in H11.
   openhyp.
@@ -315,7 +305,6 @@ Theorem return_zero_top_ok : moduleOk return_zero_top.
 
   hiding ltac:(step auto_ext).
 
-  NoDup.
   sep_auto.
   sep_auto.
 
@@ -349,4 +338,5 @@ Theorem return_zero_top_ok : moduleOk return_zero_top.
 
   Grab Existential Variables.
   eauto.
+
 Qed.
